## 9. Probar los siguientes teoremas:

### a) ((P => Q) => Q) => ((Q => P) => P)

                                            ______________________________________(ax)
                                            (P => Q) => Q, Q => P, ¬P |- ¬P
                                            ______________________________________(∧i)
                                            (P => Q) => Q, Q => P, ¬P |- ¬¬Q ∧ ¬P
                                            ______________________________________(de morgan)
                                            (P => Q) => Q, Q => P, ¬P |- ¬(¬Q ∨ P)
    ___________________________________(ax) ______________________________________(eqiv.)
    (P => Q) => Q, Q => P, ¬P |- Q => P     (P => Q) => Q, Q => P, ¬P |- ¬(Q => P)
    ______________________________________________________________________________(¬e)
                        (P => Q) => Q, Q => P, ¬P |- ⊥
                        _____________________________________(pbc)
                        (P => Q) => Q, Q => P |- P
                        _____________________________________(=>i)
                        (P => Q) => Q |- (Q => P) => P
                        _____________________________________(=>i)
                        |- ((P => Q) => Q) => ((Q => P) => P)
    .


### b) (P => Q) => ((¬P => Q) => Q)

                                    ____________________________(ax) _______________________(ax)      ______________________________(ax) _________________________(ax)
                                    P => Q, ¬P => Q, P |- P => Q     P => Q, ¬P => Q, P |- P          P => Q, ¬P => Q, ¬P |- ¬P => Q     P => Q, ¬P => Q, ¬P |- ¬P
    _________________________(lem)  ________________________________________________________(=>e)     ____________________________________________________________(=>e)
    P => Q, ¬P => Q |- P ∨ ¬P                       P => Q, ¬P => Q, P |- Q                                     P => Q, ¬P => Q, ¬P |- Q
    ____________________________________________________________________________________________________________________________________(∨e)
                                                    P => Q, ¬P => Q |- Q
                                                    _______________________________(=>i)
                                                    P => Q |- (¬P => Q) => Q
                                                    _______________________________(=>i)
                                                    |- (P => Q) => ((¬P => Q) => Q)
    .
