
## 10. Demostrar las siguientes tautologías utilizando deducción natural.

### a) (P => (P => Q)) => (P => Q)

                                _________________________________(ax)   _____________________(ax)
                                P => (P => Q), P |- P => (P => Q)       P => (P => Q), P |- P
    _____________________(ax)   _____________________________________________________________(=>e)
    P => (P => Q), P |- P                           P => (P => Q), P |- P => Q             
    __________________________________________________________________________(=>e)
                            P => (P => Q), P |- Q             
                            ______________________________(=>i)
                            P => (P => Q) |- P => Q
                            ______________________________(=>i)
                            |- (P => (P => Q)) => (P => Q)
    .


### b) (R => ¬Q) => ((R ∧ Q) => P)

                            ________________________(ax)    __________________(ax)
                            R => ¬Q, R, Q |- R => ¬Q        R => ¬Q, R, Q |- R
    __________________(ax)  __________________________________________________(=>e)
    R => ¬Q, R, Q |- Q                      R => ¬Q, R, Q |- ¬Q
    ___________________________________________________________(¬e)
                R => ¬Q, R, Q |- ⊥
                ______________________________(⊥e)
                R => ¬Q, R, Q |- P
                ______________________________(=>i)
                R => ¬Q |- R => Q => P
                ______________________________(adj.)
                R => ¬Q |- (R ∧ Q) => P
                ______________________________(=>i)
                |- (R => ¬Q) => ((R ∧ Q) => P)
    .


### c) ((P => Q) => (R => ¬Q)) => ¬(R ∧ Q)       

                                                                                                                                                            ________________________________________(ax)
                                                                                                                                                            (P => Q) => (R => ¬Q), R ∧ Q, P |- R ∧ Q
                                                                                                                                                            ________________________________________(∧e2)
                                                                                                                                                            (P => Q) => (R => ¬Q), R ∧ Q, P |- Q
                                                    _____________________________________(ax)   _____________________________________________________(ax)   ________________________________________(=>i)
                                                    (P => Q) => (R => ¬Q), R ∧ Q |- R ∧ Q       (P => Q) => (R => ¬Q), R ∧ Q |- (P => Q) => (R => ¬Q)       (P => Q) => (R => ¬Q), R ∧ Q |- P => Q
    _____________________________________(ax)       _____________________________________(∧e1)  ____________________________________________________________________________________________________(=>e)
    (P => Q) => (R => ¬Q), R ∧ Q |- R ∧ Q           (P => Q) => (R => ¬Q), R ∧ Q |- R                                            (P => Q) => (R => ¬Q), R ∧ Q |- R => ¬Q                                                                             
    _____________________________________(∧e2)      ____________________________________________________________________________________________________________________(=>e)
    (P => Q) => (R => ¬Q), R ∧ Q |- Q                                                       (P => Q) => (R => ¬Q), R ∧ Q |- ¬Q
    __________________________________________________________________________________________________________________________(¬e)
                                        (P => Q) => (R => ¬Q), R ∧ Q |- ⊥
                                        ______________________________________(¬i)
                                        (P => Q) => (R => ¬Q) |- ¬(R ∧ Q)
                                        ______________________________________(=>i)
                                        |- ((P => Q) => (R => ¬Q)) => ¬(R ∧ Q)
    .
