## 11. Probar que los siguientes secuentes son válidos sin usar principios de razonamiento clásicos

### a) (P ∧ Q) ∧ R, S ∧ T |- Q ∧ S

### b) (P ∧ Q) ∧ R |- P ∧ (Q ∧ R)

### c) P => (P => Q), P |- Q

### d) Q => (P => R), ¬R, Q |- ¬P

### e) |- (P ∧ Q) => P

### f) P => ¬Q, Q |- ¬P

### g) P => Q |- (P ∧ R) => (Q ∧ R)

### h) Q => R |- (P ∨ Q) => (P ∨ R)

### i) (P ∨ Q) ∨ R |- P ∨ (Q ∨ R)

### j) P ∧ (Q ∨ R) |- (P ∧ Q) ∨ (P ∧ R)

### k) (P ∧ Q) ∨ (P ∧ R) |- P ∧ (Q ∨ R)

### l) ¬P ∨ Q |- P => Q

### m) P => Q, P => ¬Q |- ¬P

### n) P => (Q => R), P, ¬R |- ¬Q
